prove invariant on capacity

concurrency/hack-hash-table/ResourceStateMachine.i.dfy
@@ -172,10 +172,53 @@ module ResourceStateMachine {
         :: InsertionNotPastKey(table, e, j, k))
   }
 
+  function InfoQuantity(s: Option<HT.Info>) : nat {
+    if s.None? then 0 else (
+      (if s.value.state.Inserting? then 1 else 0) +
+      (if s.value.state.RemoveTidying? || s.value.entry.Full? then 1 else 0)
+    )
+  }
+
+  function {:opaque} TableQuantity(s: seq<Option<HT.Info>>) : nat {
+    if s == [] then 0 else TableQuantity(s[..|s|-1]) + InfoQuantity(s[|s| - 1])
+  }
+
   predicate Inv(s: Variables)
   {
     && s.R?
     && InvTable(s.table)
+    && TableQuantity(s.table) + s.insert_capacity == HT.Capacity()
+  }
+
+  lemma TableQuantity_replace1(s: seq<Option<HT.Info>>, s': seq<Option<HT.Info>>, i: int)
+  requires 0 <= i < |s| == |s'|
+  requires forall j | 0 <= j < |s| :: i != j ==> s[j] == s'[j]
+  ensures TableQuantity(s') == TableQuantity(s) + InfoQuantity(s'[i]) - InfoQuantity(s[i])
+  {
+    reveal_TableQuantity();
+    if i == |s| - 1 {
+      assert s[..|s|-1] == s'[..|s|-1];
+    } else {
+      TableQuantity_replace1(s[..|s|-1], s'[..|s'|-1], i);
+    }
+  }
+
+  lemma TableQuantity_replace2(s: seq<Option<HT.Info>>, s': seq<Option<HT.Info>>, i: int)
+  requires 0 <= i < |s| == |s'|
+  requires |s| > 1
+  requires
+      var i' := (if i == |s| - 1 then 0 else i + 1);
+      forall j | 0 <= j < |s| :: i != j && i' != j ==> s[j] == s'[j]
+  ensures
+      var i' := (if i == |s| - 1 then 0 else i + 1);
+    TableQuantity(s') == TableQuantity(s)
+        + InfoQuantity(s'[i]) - InfoQuantity(s[i])
+        + InfoQuantity(s'[i']) - InfoQuantity(s[i'])
+  {
+    var s0 := s[i := s'[i]];
+    TableQuantity_replace1(s, s0, i);
+    var i' := (if i == |s| - 1 then 0 else i + 1);
+    TableQuantity_replace1(s0, s', i');
   }
 
   function {:opaque} get_empty_cell(table: seq<Option<HT.Info>>) : (e: int)
@@ -188,6 +231,25 @@ module ResourceStateMachine {
     e'
   }
 
+  lemma get_empty_cell_other_than_insertion_cell_table(table: seq<Option<HT.Info>>)
+  returns (e: int)
+  requires Complete(table)
+  requires TableQuantity(table) < |table|
+  ensures 0 <= e < |table| && table[e].Some? && table[e].value.entry.Empty?
+        && !table[e].value.state.RemoveTidying?
+        && !table[e].value.state.Inserting?
+  {
+    reveal_TableQuantity();
+    e := |table| - 1;
+    if table[e].value.entry.Empty?
+        && !table[e].value.state.RemoveTidying?
+        && !table[e].value.state.Inserting? {
+      return;
+    } else {
+      e := get_empty_cell_other_than_insertion_cell_table(table[..|table| - 1]);
+    }
+  }
+
   lemma get_empty_cell_other_than_insertion_cell(s: Variables)
   returns (e: int)
   requires Inv(s)
@@ -195,6 +257,7 @@ module ResourceStateMachine {
         && !s.table[e].value.state.RemoveTidying?
         && !s.table[e].value.state.Inserting?
   {
+    e := get_empty_cell_other_than_insertion_cell_table(s.table);
   }
 
   lemma ProcessInsertTicket_PreservesInv(s: Variables, s': Variables, insert_ticket: HT.Ticket)
@@ -221,6 +284,9 @@ module ResourceStateMachine {
       assert InsertionNotPastKey(s.table, e, j, k);
       assert ValidHashInSlot(s.table, e, j);
     }
+
+    var h := HT.hash(insert_ticket.input.key) as int;
+    TableQuantity_replace1(s.table, s'.table, h);
   }
 
   lemma InsertSkip_PreservesInv(s: Variables, s': Variables, pos: nat)
@@ -285,6 +351,8 @@ module ResourceStateMachine {
       assert InsertionNotPastKey(s.table, e, j, k);
       assert ValidHashInSlot(s.table, e, j);
     }
+
+    TableQuantity_replace2(s.table, s'.table, pos);
   }
 
   lemma InsertSwap_PreservesInv(s: Variables, s': Variables, pos: nat)
@@ -338,6 +406,8 @@ module ResourceStateMachine {
       assert ValidHashOrdering(s.table, e, pos, i);
       //assert ValidHashOrdering(s.table, e, i, pos);
     }
+
+    TableQuantity_replace2(s.table, s'.table, pos);
   }
 
   lemma InsertDone_PreservesInv(s: Variables, s': Variables, pos: nat)
@@ -436,6 +506,8 @@ module ResourceStateMachine {
       //assert ValidHashOrdering(s.table, pos, k, j);
 
     }
+
+    TableQuantity_replace1(s.table, s'.table, pos);
   }
 
   lemma InsertUpdate_PreservesInv(s: Variables, s': Variables, pos: nat)
@@ -460,6 +532,8 @@ module ResourceStateMachine {
     {
       assert InsertionNotPastKey(s.table, e, j, k);
     }
+
+    TableQuantity_replace1(s.table, s'.table, pos);
   }
 
   lemma ProcessQueryTicket_PreservesInv(s: Variables, s': Variables, query_ticket: HT.Ticket)
@@ -486,6 +560,9 @@ module ResourceStateMachine {
     {
       assert InsertionNotPastKey(s.table, e, j, k);
     }
+
+    var h := HT.hash(query_ticket.input.key) as int;
+    TableQuantity_replace1(s.table, s'.table, h);
   }
 
   lemma QuerySkip_PreservesInv(s: Variables, s': Variables, pos: nat)
@@ -518,6 +595,8 @@ module ResourceStateMachine {
     {
       assert InsertionNotPastKey(s.table, e, j, k);
     }
+
+    TableQuantity_replace2(s.table, s'.table, pos);
   }
 
   lemma QueryDone_PreservesInv(s: Variables, s': Variables, pos: nat)
@@ -542,6 +621,8 @@ module ResourceStateMachine {
     {
       assert InsertionNotPastKey(s.table, e, j, k);
     }
+
+    TableQuantity_replace2(s.table, s'.table, pos);
   }
 
   lemma QueryNotFound_PreservesInv(s: Variables, s': Variables, pos: nat)
@@ -566,6 +647,8 @@ module ResourceStateMachine {
     {
       assert InsertionNotPastKey(s.table, e, j, k);
     }
+
+    TableQuantity_replace2(s.table, s'.table, pos);
   }
 
   lemma ProcessRemoveTicket_PreservesInv(s: Variables, s': Variables, remove_ticket: HT.Ticket)
@@ -592,6 +675,9 @@ module ResourceStateMachine {
     {
       assert InsertionNotPastKey(s.table, e, j, k);
     }
+
+    var h := HT.hash(remove_ticket.input.key) as int;
+    TableQuantity_replace1(s.table, s'.table, h);
   }
 
   lemma RemoveSkip_PreservesInv(s: Variables, s': Variables, pos: nat)
@@ -624,6 +710,8 @@ module ResourceStateMachine {
     {
       assert InsertionNotPastKey(s.table, e, j, k);
     }
+
+    TableQuantity_replace2(s.table, s'.table, pos);
   }
 
   lemma RemoveFoundIt_PreservesInv(s: Variables, s': Variables, pos: nat)
@@ -648,6 +736,8 @@ module ResourceStateMachine {
     {
       assert InsertionNotPastKey(s.table, e, j, k);
     }
+
+    TableQuantity_replace2(s.table, s'.table, pos);
   }
 
   lemma RemoveTidy_PreservesInv(s: Variables, s': Variables, pos: nat)
@@ -708,6 +798,8 @@ module ResourceStateMachine {
       assert InsertionNotPastKey(s.table, e, pos', k);
       assert InsertionNotPastKey(s.table, e, j, pos');
     }
+
+    TableQuantity_replace2(s.table, s'.table, pos);
   }
 
   lemma RemoveDone_PreservesInv(s: Variables, s': Variables, pos: nat)
@@ -849,6 +941,8 @@ module ResourceStateMachine {
       assert InsertionNotPastKey(s.table, e', j, k);
       //assert InsertionNotPastKey(s.table, e', pos', j);
     }
+
+    TableQuantity_replace2(s.table, s'.table, pos);
   }
 
 }
